State the phinode postcond soundness

coq/def/Postcond.v
@@ -454,39 +454,39 @@ Module Phinode.
      Expr.value (ValueT.lift Tag.previous (get_rhs a))).
 End Phinode.
 
-Definition get_br_cond
+Definition add_terminator_cond_lessdef
            (term:terminator)
-           (l_to:l): ExprPairSet.t :=
-  let sz := Size.One in
+           (l_to:l)
+           (inv0:ExprPairSet.t): ExprPairSet.t :=
   match term with
-    | insn_br _ v l1 l2 =>
-      let cond_val := if (l_dec l_to l1) then 1%Z else 0%Z in
-      let expr1 := Expr.value (ValueT.lift Tag.physical v) in
-      let expr2 := Expr.value
-                     (ValueT.const (const_int sz (INTEGER.of_Z (Size.to_Z sz) cond_val true))) in
-      ExprPairSet.add
-        (expr1, expr2)
-        (ExprPairSet.singleton (expr2, expr1))
-    | _ => ExprPairSet.empty
+  | insn_br _ v l1 l2 =>
+    let cond_val := if (l_dec l_to l1) then 1%Z else 0%Z in
+    let expr1 := Expr.value (ValueT.lift Tag.physical v) in
+    let expr2 := Expr.value
+                   (ValueT.const (const_int Size.One (INTEGER.of_Z (Size.to_Z Size.One) cond_val true))) in
+    ExprPairSet.add
+      (expr1, expr2)
+      (ExprPairSet.add (expr2, expr1) inv0)
+  | _ => inv0
   end.
 
-Definition postcond_branch
-           (blocks_src blocks_tgt:blocks)
-           (l_from l_to:l)
-           (inv:Invariant.t): Invariant.t :=
-  match lookupAL _ blocks_src l_from, lookupAL _ blocks_tgt l_from with
-    | Some (stmts_intro _ _ term_src), Some (stmts_intro _ _ term_tgt) =>
-      let inv1 :=
-          Invariant.update_src
-            (Invariant.update_lessdef
-               (ExprPairSet.union (get_br_cond term_src l_to))) inv in
-      let inv2 :=
-          Invariant.update_tgt
-            (Invariant.update_lessdef
-               (ExprPairSet.union (get_br_cond term_tgt l_to))) inv1 in
-      inv2
-    | _, _ => inv
-  end.
+Definition add_terminator_cond
+           (inv0:Invariant.t)
+           (term_src term_tgt:terminator)
+           (l_to:l): Invariant.t :=
+  let inv1 :=
+      Invariant.update_src
+        (Invariant.update_lessdef
+           (add_terminator_cond_lessdef term_src l_to))
+        inv0
+  in
+  let inv2 :=
+      Invariant.update_tgt
+        (Invariant.update_lessdef
+           (add_terminator_cond_lessdef term_tgt l_to))
+        inv1
+  in
+  inv2.
 
 Definition postcond_phinodes_add_lessdef
            (assigns:list Phinode.assign)
